nola/examples/rust_halt/verify/mutlist_more.v
@@ -1,0 +1,114 @@
+(** * More on [mutlist] *)
+
+From nola.examples.rust_halt Require Export verify.mutlist ptrs_more sum_more
+  core.
+
+Implicit Type (X : xty) (v : val).
+
+Section mutlist.
+  Context `{!rust_haltGS CON Σ, !rust_haltC CON, !rust_haltJ CON JUDG Σ,
+    !Csem CON JUDG Σ, !Jsem JUDG (iProp Σ), !rust_haltCS CON JUDG Σ,
+    !rust_haltJS CON JUDG Σ}.
+
+  (** [iter_mutlist]: Iterate over [mutlist] *)
+  Definition iter_mutlist (sz : nat) : val := rec: "self" ["f"; "l"] :=
+    case! !"l" of [
+      #☠;
+      "f" ["l" +ₗ #1 +ₗ #0];; "self" ["f"; !("l" +ₗ #1 +ₗ #sz)]
+    ].
+
+  (** Predicate transformer for [type_iter_mutlist_mut] *)
+  Section pre_iter_mutlist_mut.
+    Context {X Yl} (pre : xpred Yl → xpred ((X *'ₓ X) :: Yl)) (post : xpred Yl).
+    Fixpoint pre_iter_mutlist_mut (xt xt' : bin X) (yl : xlist Yl) : Prop :=
+      match xt with
+      | BinLeaf => xt' = BinLeaf → post yl
+      | BinNode x xtl xtr => ∀ x' xtl' xtr', xt' = BinNode x' xtl' xtr' →
+          pre (λ yl, xtr' = xtr → pre_iter_mutlist_mut xtl xtl' yl)
+            ((x, x')', yl)'
+      end.
+    Definition pre_iter_mutlist_mut' : xpred ((binₓ X *'ₓ binₓ X) :: Yl) :=
+      λ '((xt, xt')', yl)', pre_iter_mutlist_mut xt xt' yl.
+  End pre_iter_mutlist_mut.
+
+  (** Iterate via a mutable reference to a list *)
+  Lemma type_iter_mutlist_mut {Yl}
+    `(!Ty (X:=X) T, !TyOp T κ, !LftIncl κ α, !LftIncl κ β,
+      !Closed [] (of_val f),
+      !Proper (pointwise_relation _ impl ==> pointwise_relation _ impl) pre)
+    {Γ p} :
+    α ⊑□ β -∗
+    (∀ q, type (Yl:=Yl) κ (q ◁ ty_mutref α T ᵖ:: Γ) (f [q]) (λ _, Γ) pre) -∗
+      type κ (p ◁ ty_mutref α (ty_mutlist β T) ᵖ:: Γ)
+        (iter_mutlist (ty_size T) [of_val f; p]) (λ _, Γ)
+        (pre_iter_mutlist_mut' pre).
+  Proof.
+    iIntros "#⊑ #f".
+    iAssert (∀ n p,
+      type κ (p ◁ ty_mutref α (ty_mutlist β T) ᵖ:: Γ)
+        (iter_mutlist (ty_size T) [of_val f; p]) (λ _, Γ)
+        (λ post '((xt, xt')', yl)', length (bin_lefts xt) = n ∧
+          pre_iter_mutlist_mut pre post xt xt' yl)%type)%I
+        as "Goal"; last first.
+    { iApply type_pre; last first.
+      { iApply (type_real p nat (pre_iter_mutlist_mut' pre)). iIntros (n).
+        iApply "Goal". } { done. } }
+    clear p. iIntros (n p). iInduction n as [|n] "IH" forall (p).
+    { iApply type_pre; last first.
+      { type_path p as (v). iApply type_call.
+        iApply (type_mutref_subty v);
+          [|iApply (subty_mutlist_unfold (T:=T))|
+            iApply (subty_mutlist_fold (T:=T))|].
+        { move=> ?. exact bin_unwrap_wrap. }
+        iApply (type_case_sum_mutref v); [|by iApply type_false].
+        iApply (type_leak ᵖ[_]). iApply type_value. }
+      move=>/= ?[[[|???]?]?]/=[? to]//[] /(f_equal bin_wrap)/=.
+      rewrite bin_wrap_unwrap=> ? _. exact: to. }
+    iApply type_pre; last first.
+    { type_path p as (v). iApply type_call.
+      iApply (type_mutref_subty v);
+        [|iApply (subty_mutlist_unfold (T:=T))|
+          iApply (subty_mutlist_fold (T:=T))|].
+      { move=> ?. exact bin_unwrap_wrap. }
+      iApply (type_case_sum_mutref v); [by iApply type_false|].
+      iApply type_mutref_prod_split. iApply type_seq.
+      { iApply (type_frame ᵖ[_]); [|by iApply "f"].
+        apply: tcx_extract_cons; [|exact _]. exact: etcx_extract_tl. }
+      iIntros (?). type_bind (!_)%E; [by iApply type_deref_mutref_mutref|].
+      iIntros (v'). iApply type_subty; [|by iApply "IH"].
+      iApply (subty_mutref_lft (T:=ty_mutlist _ T)).
+      iApply lft_sincl_meet_intro; by [iApply lft_sincl_refl|]. }
+    move=>/= ?[[[|???]?]?]/=[leq to]//=[?[??]] /(f_equal bin_wrap)/=.
+    rewrite bin_wrap_unwrap=> eq. move: (to _ _ _ eq). apply Proper0=> ? H eq'.
+    move: (H eq')=> ?. split=>//. by case: leq.
+  Qed.
+
+  (** Lemma for [type_iter_mutlist_mut_fun] *)
+  Lemma pre_iter_mutlist_mut_fun {X Yl} (g : X → X) {post xt xt' yl} :
+    @pre_iter_mutlist_mut X Yl
+      (λ post '((x, x')', yl)', x' = g x → post yl) post xt xt' yl ↔
+      (xt' = bin_lspine_map g xt → post yl).
+  Proof.
+    move: xt' yl. elim: xt=>//= ?? IH ? _ xt' yl. split.
+    - case: xt'=>//= ??? H [???]. subst. eapply IH; [exact: H|done].
+    - move=> H ??????. subst. apply IH=> ?. apply H. by f_equal.
+  Qed.
+  (** [type_iter_mutlist_mut] over a typical predicate transformer that resolves
+    the prophecy by some function *)
+  Lemma type_iter_mutlist_mut_fun {X} (g : X → X) {Yl}
+    `(!Ty (X:=X) T, !TyOp T κ, !LftIncl κ α, !LftIncl κ β,
+      !Closed [] (of_val f)) {Γ p} :
+    α ⊑□ β -∗
+    (∀ q, type (Yl:=Yl) κ
+      (q ◁ ty_mutref α T ᵖ:: Γ) (f [q]) (λ _, Γ)
+        (λ post '((x, x')', yl)', x' = g x → post yl)%type) -∗
+      type κ (p ◁ ty_mutref α (ty_mutlist β T) ᵖ:: Γ)
+        (iter_mutlist (ty_size T) [of_val f; p]) (λ _, Γ)
+          (λ post '((xt, xt')', yl)', xt' = bin_lspine_map g xt → post yl)%type.
+  Proof.
+    iIntros "#⊑ type". iApply type_pre; last first.
+    { iApply (type_iter_mutlist_mut with "⊑ type"). move=>/= ?? to ? H ?.
+      by apply to, H. }
+    by move=>/= > /pre_iter_mutlist_mut_fun.
+  Qed.
+End mutlist.
