README.md
@@ -226,3 +226,5 @@ All the Coq code is in [`nola/`](nola/) and structured as follows:
           type)
       - [`mutlist`](nola/examples/rust_halt/verify/mutlist.v) (Singly linked
           list over a mutable reference),
+        [`mutlist_more`](nola/examples/rust_halt/verify/mutlist_more.v) (More on
+          `mutlist`)
